kuiops/sdpa/Kuiops.Sdpa.Flash.Kf.fsti
@@ -33,7 +33,7 @@ open Kuiper.TensorRO { vtlayout_of_tlayout }
 inline_for_extraction noextract
 fn sdpa_flash_kf
   (#et_ab #et_acc : Type0)
-  {| scalar et_acc |} {| floating et_acc |} {| real_like et_acc |}
+  {| floating et_acc |} {| real_like et_acc |}
   {| scalar et_ab |} {| real_like et_ab |}
   {| FC.float_cast et_ab et_acc |}
   {| FC.float_cast et_acc et_ab |}
