kuiops/sdpa/Kuiops.Sdpa.Flash.KfSub.fsti
@@ -68,7 +68,7 @@ let jt_rest
 inline_for_extraction noextract
 fn sdpa_flash_jt_body
   (#et_ab #et_acc : Type0)
-  {| scalar et_acc |} {| floating et_acc |} {| real_like et_acc |}
+  {| floating et_acc |} {| real_like et_acc |}
   {| scalar et_ab |} {| real_like et_ab |}
   {| FC.float_cast et_ab et_acc |}
   {| FC.float_cast et_acc et_ab |}
